lean4/Main.lean
@@ -1,22 +1,5 @@
 import «Le»
 
--- def onePlusOneIsThree : 1 + 1 = 3 := rfl
-def onePlusOneIsTwo : 1 + 1 = 2 := by
-  simp
-
-theorem add : 1 + 1 = 2 := by
-  simp
-
-theorem append : "Str".append "ing" = "String" := by
-  rfl
-
--- theorem andImpliesOr : A ∧ B → A ∨ B :=
---   fun andEvidence =>
---     match andEvidence with
---     | And.intro a _ => Or.inl a
-
 def main : IO Unit := do
-  -- IO.println s!"Hello, {hello}!"
-  -- let n := fib 40
-  -- IO.println s!"fib 40 = {n}!"
-  IO.println s!"pi = {leibniz 10000000 0.0}!"
+  IO.println s!"fib 20 = {fib 20} ."
+  IO.println s!"pi = {leibniz 10000000} ."
